src/lowparse/LowParse.SLow.Sum.fst
@@ -1,0 +1,69 @@
+module LowParse.SLow.Sum
+include LowParse.Spec.Sum
+include LowParse.SLow.Enum
+
+module B32 = FStar.Bytes
+module U32 = FStar.UInt32
+
+#set-options "--z3rlimit 16"
+
+inline_for_extraction
+let parse32_sum_gen
+  (#kt: parser_kind)
+  (t: sum)
+  (#p: parser kt (sum_repr_type t))
+  (p32: parser32 (parse_enum_key p (sum_enum t)))
+  (#k: parser_kind)
+  (#pc: ((x: sum_key t) -> Tot (parser k (sum_cases t x))))
+  (pc32: ((x: sum_key t) -> Tot (parser32 (pc x))))
+: Tot (parser32 (parse_sum t p pc))
+= fun (input: bytes32) -> ((
+    match p32 input with
+    | Some (tg, consumed_tg) ->
+      let input' = b32slice input consumed_tg (B32.len input) in 
+      begin match pc32 tg input' with
+      | Some (d, consumed_d) ->
+        // FIXME: implicit arguments are not inferred because (synth_tagged_union_data ...) is Tot instead of GTot
+        assert (parse (parse_synth #_ #_ #(sum_type t) (pc tg) (synth_tagged_union_data (sum_tag_of_data t) tg)) (B32.reveal input') == Some (d, U32.v consumed_d));
+        Some (d, U32.add consumed_tg consumed_d)
+      | _ -> None
+      end
+    | _ -> None
+  )
+  <: (res: option (sum_type t * U32.t) { parser32_correct (parse_sum t p pc) input res } )
+  )
+
+(*
+module Seq = FStar.Seq
+
+#set-options "--z3rlimit 32"
+
+let parse32_sum_gen_correct
+  (#kt: parser_kind)
+  (t: sum)
+  (#p: parser kt (sum_repr_type t))
+  (p32: parser32 (parse_enum_key p (sum_enum t)))
+  (#k: parser_kind)
+  (#pc: ((x: sum_key t) -> Tot (parser k (sum_cases t x))))
+  (pc32: ((x: sum_key t) -> Tot (parser32 (pc x))))
+  (input: bytes32)
+: Lemma
+  (parser32_correct (parse_sum t p pc) input (parse32_sum_gen' t p32 pc32 input))
+=  match p32 input with
+  | Some (tg, consumed_tg) ->
+    assert (parse (parse_enum_key p (sum_enum t)) (B32.reveal input) == Some (tg, U32.v consumed_tg));
+    let input' = b32slice input consumed_tg (B32.len input) in
+    assert (B32.reveal input' == Seq.slice (B32.reveal input) (U32.v consumed_tg) (B32.length input));
+    let ptg : parser k (refine_with_tag (sum_tag_of_data t) tg) = pc tg in
+    begin match pc32 tg input' with
+    | Some (d, consumed_d) ->
+      assert (parse ptg (B32.reveal input') == Some (d, U32.v consumed_d));
+      // FIXME: implicit arguments are not inferred because (synth_tagged_union_data ...) is Tot instead of GTot
+      assert (parse (parse_synth #_ #_ #(sum_type t) ptg  (synth_tagged_union_data (sum_tag_of_data t) tg)) (B32.reveal input') == Some (d, U32.v consumed_d));
+      ()
+    | None -> 
+      assert (parse ptg (B32.reveal input') == None);
+      ()
+    end
+  | None -> ()
+
